Charge!/src/Charge/Tactics/Lists/Fold.v
@@ -2,6 +2,7 @@ Require Import MirrorCore.TypesI.
 Require Import MirrorCore.Lambda.AppN.
 Require Import MirrorCore.Lambda.Red.
 Require Import MirrorCore.Lambda.RedAll.
+Require Import MirrorCore.Lambda.Expr.
 Require Import MirrorCore.RTac.Simplify.
 
 Require Import Charge.ModularFunc.BaseFunc.
@@ -9,6 +10,7 @@ Require Import Charge.ModularFunc.ListFunc.
 Require Import Charge.ModularFunc.BaseType.
 Require Import Charge.ModularFunc.ListType.
 Require Import Charge.ModularFunc.SemiEqDecTyp.
+Require Import Charge.ModularFunc.Denotation.
 
 Require Import ExtLib.Core.RelDec.
 
@@ -27,6 +29,8 @@ Section Fold.
   Context {RTypeOk_typ : RTypeOk}.
   Context {RSymOk_func : RSymOk RSym_func}.
   Context {Typ2Ok_Fun : Typ2Ok Typ2_Fun}.
+Check typ2_match.
+SearchAbout typ2_match.
 
   Definition foldTac (e : expr typ func) (args : list (expr typ func)) : expr typ func :=
     match listS e with
@@ -39,9 +43,12 @@ Section Fold.
 		  	      | Some pf => 
                     fold_right (fun x acc => beta (beta (App (App f (mkConst u x)) acc))) acc 
                        (listD (eq_rect _ typD lst _ pf))
-		  	      | None => apps e args
-		  	    end
-              | _ => apps e args
+                  | None => apps e args
+                end
+		  	  | Some _ => apps e args
+		  	  | None => 
+		  	    let (lst', e') := expr_to_list lst in
+		  	      fold_right (fun x acc => beta (beta (App (App f x) acc))) (apps e (f::acc::e'::nil)) lst'
             end
           | _ => apps e args
         end
@@ -62,6 +69,11 @@ Require Import ExtLib.Tactics.
         let H1 := fresh "H" in let H2 := fresh "H" in
           apply typ2_inj in H as [H1 H2]; [unfold Rty in H1, H2; r_inj H1; r_inj H2 | apply _] |
         repeat subst].
+  
+  Ltac list_inj :=
+    match goal with
+      | H : tyList _ = tyList _ |- _ => apply tyList_inj in H; unfold Rty in H; subst
+    end.
  Context {Expr_typ : Expr RType_typ (expr typ func)}.
 
 Check Typ2Ok_Fun.
@@ -69,7 +81,6 @@ Check Typ2Ok_Fun.
     (H : ExprDsimul.ExprDenote.exprD' tus tvs t e = Some df) :
     ExprDsimul.ExprDenote.exprD' tus tvs t (beta e) = Some df.
   Proof.
-
     pose proof (beta_sound tus tvs e t).
     rewrite H in H0.
     forward; inv_all; subst. 
@@ -78,48 +89,111 @@ Check Typ2Ok_Fun.
     do 2 (apply functional_extensionality; intro).
     symmetry; apply H1.
   Qed.
+
+  Lemma Rcast_option_inj (t u : typ) r (a : typD t) (b : typD u)
+    (H : Rcast option r (Some a) = Some b) :
+    b = Rcast id r a.
+  Proof.
+    clear -H.
+    unfold Rcast, Relim, Rsym, eq_sym in *.
+    destruct r; inv_all; subst. reflexivity.
+  Qed.
+
+  Lemma Rcast_id t f : 
+    Rcast id (Rrefl t) f = f.
+  Proof.
+    reflexivity.
+  Qed.
+
+Ltac run_forward_step H1 H2 type_tac expr_tac :=
+  let H := fresh "H" in 
+      pose proof type_tac as H; r_inj H; pose proof expr_tac; subst;
+      clear H1 H2.
+
+Ltac lf_forward_step :=
+  match goal with 
+    | H : Some _ = listS _ |- _ =>  symmetry in H
+    | H : typ2 _ _ = typ2 _ _ |- _ => r_inj H; clear_eq
+    | H : Rty (typ2 _ _) (typ2 _ _) |- _ => r_inj H; clear_eq
+    | H : Rcast option _ (Some _) = Some _ |- _ => apply Rcast_option_inj in H; subst
+	| H1 : listS ?e = Some (pNil _), H2 : ExprDsimul.ExprDenote.exprD' _ _ _ ?e = Some _|- _ =>
+	  let H := fresh "H" in
+	     pose proof (lf_nil_type_eq _ _ H1 H2) as H; r_inj H; pose proof(lf_nil_eq _ H1 H2); subst;
+	     clear H1 H2
+	| H1 : listS ?e = Some (pFold _ _), H2 : ExprDsimul.ExprDenote.exprD' _ _ _ ?e = Some _|- _ =>
+	  let H := fresh "H" in
+	     pose proof (lf_fold_type_eq _ _ H1 H2) as H; r_inj H; pose proof(lf_fold_eq _ H1 H2); subst;
+	     clear H1 H2
+    | _ => 
+       first [
+        progress (unfold foldD, fun_to_typ3 in *) |
+        progress (repeat rewrite (exprT_App_wrap) in *)
+      ]
+  end.
+ 
+Ltac lf_fold_step :=
+  match goal with
+    | H2 : ExprDsimul.ExprDenote.exprD' ?tus ?tvs
+       (typ2 (typ2 ?u (typ2 ?t ?t)) (typ2 ?t (typ2 (tyList ?u) ?t))) ?e =
+     Some (fun _ _ => foldD ?t ?u) |- _ => fail 1
+	| H1 : listS ?e = Some (pFold _ _), H2 : ExprDsimul.ExprDenote.exprD' _ _ _ ?e = Some _|- _ =>
+	  let H := fresh "H" in
+	     pose proof (lf_fold_type_eq _ _ H1 H2) as H; r_inj H; repeat clear_eq; pose proof(lf_fold_eq _ H1 H2); subst
+  end.
+
+  
+Ltac bf_forward_step :=
+  match goal with 
+    | H : Some _ = baseS _ |- _ =>  symmetry in H
+	| H1 : baseS ?e = Some (pConst _ _), H2 : ExprDsimul.ExprDenote.exprD' _ _ _ ?e = Some _|- _ =>
+	  let H := fresh "H" in
+	     pose proof (bf_const_type_eq _ _ H1 H2) as H; r_inj H; repeat clear_eq; pose proof(bf_const_eq _ H1 H2); subst;
+	     clear H1 H2
+  end.
   
   Lemma foldTacOk : partial_reducer_ok foldTac.
   Proof.
     unfold partial_reducer_ok; intros.
+    exists val; split; [|reflexivity].
     unfold foldTac.
-    remember (listS e); destruct o; [| exists val; tauto].
-    destruct l; try (exists val; tauto).
-    destruct es; try (exists val; tauto).
-    destruct es; try (exists val; tauto).
-    destruct es; try (exists val; tauto).
-    destruct es; try (exists val; tauto).
-    remember (baseS e2); destruct o; try (exists val; tauto).
-    destruct b; try (exists val; tauto).
+    remember (listS e); destruct o; [|assumption].
+    destruct l; try assumption.
+    destruct es; try assumption.
+    destruct es; try assumption.
+    destruct es; try assumption.
+    destruct es; try assumption.
+    simpl in H.
+    remember (baseS e2); destruct o.
+    destruct b; try assumption.
     remember (type_cast t2 (tyList t1)).
-    destruct o; [|exists val; tauto].
+    destruct o; [|assumption].
     simpl in H.
     autorewrite with exprD_rw in H; simpl in H; forward; inv_all; subst.
     autorewrite with exprD_rw in H0; simpl in H0; forward; inv_all; subst.
     autorewrite with exprD_rw in H2; simpl in H2; forward; inv_all; subst.
+Check @lf_fold_eq.
+
+	lf_forward_step.
+	lf_fold_step.
+	lf_fold_step.
+  match goal with
+    | H2 : ExprDsimul.ExprDenote.exprD' ?tus ?tvs
+       (typ2 (typ2 ?u (typ2 ?t ?t)) (typ2 ?t (typ2 (tyList ?u) ?t))) ?e =
+     Some (fun  (_ : HList.hlist typD tus) (_ : HList.hlist typD tvs) => foldD ?t ?u) |- _ => idtac "hej"
+  end.
+	lf_fold_step.
+	progress lf_fold_step.
+	progress lf_fold_step.
+	repeat clear_eq.
+	lf_forward_step.
     unfold Rty in r; subst.
-    
-    eexists; split; [|reflexivity].
-    
     Opaque beta.
-    
+    bf_forward_step.
+    bf_forward_step.
+    clear_eq.
+    lf_forward_step.
+    lf_forward_step.
     simpl.
-    symmetry in Heqo.
-    pose proof (lf_fold_type_eq _ _ Heqo H4).
-    r_inj H6.
-    pose proof (lf_fold_eq _ Heqo H4).
-	subst.
-	unfold foldD.
-	
-	clear H4.
-	Require Import Charge.ModularFunc.Denotation.
-	unfold Denotation.fun_to_typ3.    
-	repeat rewrite exprT_App_wrap.
-	
-	Check @bf_const_type_eq.
-	symmetry in Heqo0.
-	pose proof (bf_const_eq _ Heqo0 H1).
-	subst. clear H1.	
 	remember (listD t3). clear Heql.
 	induction l; intros; subst.
 	+ simpl. assumption.
@@ -136,6 +210,114 @@ Check Typ2Ok_Fun.
       rewrite exprT_App_wrap_sym.
       rewrite exprT_App_wrap_sym.
       reflexivity.
+    + remember (expr_to_list e2).
+      destruct p.
+      clear Heqo0.
+      autorewrite with exprD_rw in H; simpl in H; forward; inv_all; subst.
+      autorewrite with exprD_rw in H0; simpl in H0; forward; inv_all; subst.
+      autorewrite with exprD_rw in H2; simpl in H2; forward; inv_all; subst.
+      autorewrite with exprD_rw in H1; simpl in H1; forward; inv_all; subst.
+      repeat lf_forward_step.
+      generalize dependent e2. induction l. simpl. intros. 
+      symmetry in Heqp. apply expr_to_list_nil in Heqp. subst.
+      
+      autorewrite with exprD_rw; simpl; forward; inv_all; subst.
+      autorewrite with exprD_rw; simpl; forward; inv_all; subst.
+      autorewrite with exprD_rw; simpl; forward; inv_all; subst.
+      forward; inv_all; subst.
+      forward; inv_all; subst.
+      autorewrite with exprD_rw; simpl; forward; inv_all; subst.
+       assumption.
+      intros.
+      symmetry in Heqp.
+      simpl.
+      apply beta_sound.
+      apply beta_sound.
+
+
+      lf_forward_step.
+      lf_forward_step.
+      lf_forward_step.
+      lf_forward_step.
+      repeat rewrite (exprT_App_wrap) in IHl.
+      
+      autorewrite with exprD_rw; simpl; forward; inv_all; subst.
+      
+      destruct (expr_to_list_cons tus tvs _ _ Heqp H) as [? [? ?]].
+      subst.
+      assert ( ExprDsimul.ExprDenote.exprD' tus tvs t0 (App (App (App e e0) e1) x) =
+      Some
+        (fun (us : HList.hlist typD tus) (vs : HList.hlist typD tvs) =>
+         fold_right (typ_to_fun2 (e8 us vs)) (e7 us vs) (listD (e5 us vs)))).
+      autorewrite with exprD_rw; simpl; forward; inv_all; subst.
+      assert (typeof_expr tus tvs x = Some (tyList t1)) by admit.
+      forward.
+      autorewrite with exprD_rw; simpl; forward; inv_all; subst.
+      autorewrite with exprD_rw; simpl; forward; inv_all; subst.
+      
+      lf_forward_step.
+      pose proof (lf_nil_func_type_eq _ _ Heqo1 H1).
+      subst.
+      rewrite H4 in *.
+      list_inj.
+      pose proof (lf_nil_func_eq _ Heqo1 H1).
+	  subst.
+	  simpl.
+	  
+	  Lemma listD_nil (t : typ) : listD (nilD t) = nil.
+	  Proof.
+	    unfold listD, nilD, eq_rect_r, eq_rect, id, eq_sym.
+	    generalize (btList t).
+	    generalize dependent (tyList t).
+	    generalize dependent (typD t).
+		intros.
+		generalize dependent (typD t0).
+		intros; subst. reflexivity.
+	  Qed.
+	  
+	  rewrite listD_nil. simpl. assumption.
+	  
+	  destruct e2_2; try assumption.
+	  destruct e2_1; try assumption.
+	  simpl.
+	  remember (listS f). destruct o; try assumption.
+	  destruct l; try assumption.
+
+	  simpl in H.
+	  autorewrite with exprD_rw in H; simpl in H; forward; inv_all; subst.
+      autorewrite with exprD_rw in H0; simpl in H0; forward; inv_all; subst.
+      autorewrite with exprD_rw in H2; simpl in H2; forward; inv_all; subst.
+      autorewrite with exprD_rw in H1; simpl in H1; forward; inv_all; subst.
+      autorewrite with exprD_rw in H11; simpl in H11; forward; inv_all; subst.
+      autorewrite with exprD_rw in H10; simpl in H10; forward; inv_all; subst.
+	  
+      lf_forward_step.
+      lf_forward_step.
+      lf_forward_step.
+      lf_forward_step.
+      lf_forward_step.
+      pose proof (lf_cons_func_type_eq _ _ Heqo1 H5).
+      Check lf_cons_func_type_eq.
+      r_inj H8.
+      pose proof (lf_cons_func_eq _ Heqo1 H5).
+	  subst.
+	  simpl.
+
+
+      lf_forward_step.
+      Print type_of_apply.
+      Check typ2_inj.
+      Print Rty.
+      Print Typ2Ok.
+      SearchAbout type_of_apply.
+      lf_forward_step.
+      lf_forward_step.
+	  
+	  unfold nilD, listD, eq_rect_r, eq_rect, eq_sym. simpl.
+	  remember (btList t2).
+	  destruct e2.      
+      lf_forward_step.
+      simpl in H.
   Qed.
 
 End Fold.
